Refactoring and documentation

VLSM/Composition.v
@@ -9,26 +9,55 @@ From CasperCBC
 
 (**
 
-** VLSM compositions and projections
-
-This section provides Coq definitions for composite VLSMs and their projections
+This module provides Coq definitions for composite VLSMs and their projections
 to components.
-
-In the sequel we will succesively define 
 *)
 
-Section indexing.
+Section VLSM_composition.
 
+(**
+* VLSM composition
+
+Let us fix a type for <<message>>s, and an <<index>> type for the VLSM components
+such that equality on <<index>> is decidable.
+
+*)
+
+  Context {message : Type}
+          {index : Type}
+          {IndEqDec : EqDec index}
+          .
+          
   Section composite_type.
 
-    Context {message : Type}
-            {index : Type}
-            {IndEqDec : EqDec index}
-            (IT : index -> VLSM_type message).
+(**
 
+** The type of a composite VLSM
+
+Let IM be a family of VLSMs indexed by <<index>> and for each index <<i>>,
+let <<IT i>> be the [VLSM_type] of VLSM <<IM i>>.  Note that all 
+[VLSM_type]s share the same type of <<message>>s.
+
+*)
+
+    Context (IT : index -> VLSM_type message).
+
+(**
+A [composite_state] is an indexed family of [state]s, yielding for each
+index <<n>> a [state] of <<IT n>>, the [VLSM_type] corresponding to <<n>>.
+
+Note that the [composite_state] type is the dependent product type of the 
+family of types <<[@state _ (IT n) | n <- index]>>.
+*)
     Definition _composite_state : Type :=
       forall n : index, (@state _ (IT n)).
 
+(**
+A [composite_label] is a pair between an index <<N>> and a [label] of <<IT n>>.
+
+Note that the [composite_label] type is the dependent sum of the family of
+types <<[@label _ (IT n) | n <- index]>>.
+*)
     Definition _composite_label
       : Type
       := sigT (fun n => @label _ (IT n)).
@@ -41,6 +70,10 @@ Section indexing.
     Definition composite_state := @state message composite_type.
     Definition composite_label := @label message composite_type.
 
+(**
+A very useful operation on [composite_state]s is updating the state corresponding
+to a component:
+*)
     Definition state_update
                (s : composite_state)
                (i : index)
@@ -53,6 +86,9 @@ Section indexing.
       | _ => s j
       end.
 
+(**
+The next few results describe several properties of the [state_update] operation.
+*)
     Lemma state_update_neq
                (s : composite_state)
                (i : index)
@@ -101,65 +137,101 @@ Section indexing.
       - repeat rewrite state_update_neq; try assumption.
         reflexivity.
     Qed.
-
   End composite_type.
 
   Section composite_sig.
+(**
 
-    Context {message : Type}
-            {index : Type}
-            {IndEqDec : EqDec index}
-            {IT : index -> VLSM_type message}
+** The signature of a composite VLSM
+
+Assume an non-empty <<index>> type (let <<i0>> be an index) and let <<IT>> be
+an <<index>>ed family of [VLSM_type]s, and for each index <<i>>, let <<IS i>> be
+a [VLSM_sign]ature of type <<IT i>>.
+*)
+
+    Context {IT : index -> VLSM_type message}
             (i0 : index)
-            (IS : forall i : index, LSM_sig (IT i)).
+            (IS : forall i : index, VLSM_sign (IT i)).
 
-    Definition _composite_initial_state_prop
+(**
+A [composite_state] has the [initial_state_prop]erty if all of its component
+states have the [initial_state_prop]erty in the corresponding component signature.
+*)
+    Definition composite_initial_state_prop
                (s : composite_state IT)
       : Prop
       :=
         forall n : index, @initial_state_prop _ _ (IS n) (s n).
 
-    Definition _composite_initial_state
-      := { s : composite_state IT | _composite_initial_state_prop s }.
+    Definition composite_initial_state
+      := { s : composite_state IT | composite_initial_state_prop s }.
 
-    Definition _composite_s0 : _composite_initial_state.
+    Definition composite_s0 : composite_initial_state.
       exists (fun (n : index) => proj1_sig (@s0 _ _ (IS n))).
       intro i. destruct s0 as [s Hs]. assumption.
     Defined.
 
-    Definition _composite_initial_message_prop (m : message) : Prop
+(**
+A message has the [initial_message_prop]erty in the [composite_sig]nature
+iff it has the [initial_message_prop]erty in any of the component signatures.
+*)
+    Definition composite_initial_message_prop (m : message) : Prop
       :=
         exists (n : index) (mi : @initial_message _ _ (IS n)), proj1_sig mi = m.
 
     (* An explicit argument for the initial state witness is no longer required: *)
-    Definition _composite_m0 : message := @m0 _ _ (IS i0).
+    Definition composite_m0 : message := @m0 _ _ (IS i0).
 
-    Definition _composite_l0 : composite_label IT
+    Definition composite_l0 : composite_label IT
       := existT _ i0 (@l0 _ _ (IS i0)) .
 
     Definition composite_sig
-      : LSM_sig (composite_type IT)
+      : VLSM_sign (composite_type IT)
       :=
-        {|   initial_state_prop := _composite_initial_state_prop
-           ; s0 := _composite_s0
-           ; initial_message_prop := _composite_initial_message_prop
-           ; m0 := _composite_m0
-           ; l0 := _composite_l0
+        {|   initial_state_prop := composite_initial_state_prop
+           ; s0 := composite_s0
+           ; initial_message_prop := composite_initial_message_prop
+           ; m0 := composite_m0
+           ; l0 := composite_l0
         |}.
+
+(**
+We can always "lift" state <<sj>> from component <<j>> to a composite state by 
+updating an initial composite state, say [s0], to <<sj>> on component <<j>>.
+*)
+    Definition lift_to_composite_state
+      (j : index)
+      (sj : @state _ (IT j))
+      (s0X := proj1_sig (@s0 _ _ composite_sig))
+      : composite_state IT
+      := state_update IT s0X j sj
+      .
 
   End composite_sig.
 
   Section composite_vlsm.
+(**
 
-    Context {message : Type}
-            {index : Type}
-            {IndEqDec : EqDec index}
-            {IT : index -> VLSM_type message}
+** Constrained VLSM composition
+
+Assume an non-empty <<index>> type (let <<i0>> be an index), let
+<<IT>> be an <<index>>ed family of [VLSM_type]s, and for each index <<i>>, let
+<<IS i>> be a [VLSM_sign]ature of type <<IT i>> and <<IM i>> be a VLSM of
+signature <<IS i>>.
+*)
+
+    Context {IT : index -> VLSM_type message}
             (i0 : index)
-            {IS : forall i : index, LSM_sig (IT i)}
+            {IS : forall i : index, VLSM_sign (IT i)}
             (IM : forall n : index, VLSM (IS n)).
 
-    Definition _composite_transition
+(**
+The [transition] function for the [composite_vlsm] is defined as follows
+takes a transition in the VLSM corresponding to the given [composite_label]
+and returnes the produced message together with the state updated on that
+component:
+*)
+    Definition composite_transition
                (l : composite_label IT)
                (som : composite_state IT * option message)
       : composite_state IT * option message
@@ -169,7 +241,12 @@ Section indexing.
       let (si', om') := transition li (s i, om) in
       (state_update IT s i si',  om').
 
-    Definition _composite_valid
+(**
+Given a [composite_label] <<(i, li)>> and a [composite_state]-message
+pair <<(s, om)>>, [free_composite_valid]ity is defined as [valid]ity in 
+the <<i>>th component <<IM i>>.
+*)
+    Definition free_composite_valid
                (l : composite_label IT)
                (som : composite_state IT * option message)
       : Prop
@@ -178,24 +255,42 @@ Section indexing.
       let (i, li) := l in
       valid li (s i, om).
 
-    (* Section 2.4.3 Constrained VLSM composition *)
+(**
+A <<constraint>> for a composite VLSM is a [valid]ity condition defined
+directly on [composite_label]s and [composite_state]s, thus being able to
+impose a global condition.
 
-    Definition _composite_valid_constrained
+[constrained_composite_valid]ity interposes such a <<constraint>> on top of
+the [free_composite_valid]ity.
+*)
+
+    Definition constrained_composite_valid
                (constraint : composite_label IT -> composite_state IT  * option message -> Prop)
                (l : composite_label IT)
                (som : composite_state IT * option message)
       :=
-        _composite_valid l som /\ constraint l som.
+        free_composite_valid l som /\ constraint l som.
 
-    Definition composite_vlsm_constrained
+    Definition composite_vlsm
                (constraint : composite_label IT -> composite_state IT * option (message) -> Prop)
       : VLSM (composite_sig i0 IS)
       :=
-        {|  transition := _composite_transition
-            ;   valid := _composite_valid_constrained constraint
+        {|  transition := composite_transition
+            ;   valid := constrained_composite_valid constraint
         |}.
 
+    Definition composite_valid
+      (constraint : composite_label IT -> composite_state IT * option (message) -> Prop)
+      := @valid _ _ _ (composite_vlsm constraint).
+
     Section constraint_subsumption.
+(**
+
+** Constraint subssumption
+
+A <<constraint1>> is subssumed by <<constraint2>> if <<constraint1> is stronger
+than <<constraint2>> for any input.
+*)
 
     Definition constraint_subsumption
         (constraint1 constraint2 : composite_label IT -> composite_state IT * option message -> Prop)
@@ -206,12 +301,22 @@ Section indexing.
     Context
       (constraint1 constraint2 : composite_label IT -> composite_state IT * option message -> Prop)
       (Hsubsumption : constraint_subsumption constraint1 constraint2)
-      (X1 := composite_vlsm_constrained constraint1)
-      (X2 := composite_vlsm_constrained constraint2)
+      (X1 := composite_vlsm constraint1)
+      (X2 := composite_vlsm constraint2)
       (S := composite_sig i0 IS)
       (T := composite_type IT)
       .
 
+(**
+Let <<X1>>, <<X2>> be two compositions of the same family of VLSMs but with 
+constraints <<constraint1>> and <<constraint2>, respectively. Further assume 
+that <<constraint1>> is subssumed by <<constraint2>>.
+
+We will show that <<X1>> is trace-included into <<X2>> by applying 
+Lemma [basic_VLSM_inclusion]
+*)
+
+(* begin hide *)
     Lemma constraint_subsumption_protocol_valid
       (l : label)
       (s : state)
@@ -240,6 +345,12 @@ Section indexing.
         apply protocol_generated_valid with _om _s; assumption.
     Qed.
 
+(* end hide *)
+
+(**
+Then <<X1>> is trace-included into <<X2>>.
+*)
+
     Lemma constraint_subsumption_incl
       : VLSM_incl X1 X2
       .
@@ -255,15 +366,14 @@ Section indexing.
 
     End constraint_subsumption.
 
-    Definition composite_transition
-      (constraint : composite_label IT -> composite_state IT * option (message) -> Prop)
-      := @transition _ _ _ (composite_vlsm_constrained constraint).
+(**
 
-    Definition composite_valid
-      (constraint : composite_label IT -> composite_state IT * option (message) -> Prop)
-      := @valid _ _ _ (composite_vlsm_constrained constraint).
+** Free VLSM composition
 
-    (* Section 2.4.3 Free VLSM composition using constraint = True *)
+The [free_constraint] is defined to be [True] for all inputs. 
+Thus, the [free_composite_vlsm] is the [composite_vlsm] using the
+[free_constraint].
+*)
 
     Definition free_constraint
                (l : composite_label IT)
@@ -272,139 +382,99 @@ Section indexing.
       :=
         True.
 
-    Definition composite_vlsm_free : VLSM (composite_sig i0 IS)
+    Definition free_composite_vlsm : VLSM (composite_sig i0 IS)
       :=
-        composite_vlsm_constrained free_constraint
+        composite_vlsm free_constraint
     .
 
+
+(**
+A component [protocol_state]'s [lift_to_composite_state] is a [protocol_state]
+for the [free_composite_vlsm].
+*)
     Lemma protocol_prop_composite_free_lift
       (S := (composite_sig i0 IS))
       (j : index)
       (sj : @state _ (IT j))
       (om : option message)
       (Hp : protocol_prop (IM j) (sj, om))
-      (s0X := proj1_sig (@s0 _ _ S))
-      : protocol_prop composite_vlsm_free ((state_update IT s0X j sj), om)
+      (s := lift_to_composite_state i0 IS j sj)
+      : protocol_prop free_composite_vlsm (s, om)
       .
     Proof.
       remember (sj, om) as sjom.
       generalize dependent om. generalize dependent sj.
-      induction Hp; intros; inversion Heqsjom; subst; clear Heqsjom.
-      - assert (Hinit : @initial_state_prop _ _ S (state_update IT s0X j s)).
-        { intro i.
+      induction Hp; intros; inversion Heqsjom; subst; clear Heqsjom
+      ; unfold s0; clear s0.
+      - assert (Hinit : @initial_state_prop _ _ S (lift_to_composite_state i0 IS j s)).
+        { intro i. unfold lift_to_composite_state.
           destruct (eq_dec i j).
           - subst; rewrite state_update_eq. unfold s. destruct is. assumption.
           - rewrite state_update_neq; try assumption.
-            destruct (@s0 _ _ S) as [s00 Hinit].
-            unfold s0X; clear s0X; simpl.
+            destruct @Common.s0 as [s00 Hinit].
+            simpl.
             apply Hinit.
         }
-        remember (exist (@initial_state_prop _ _ S) (state_update IT s0X j s) Hinit) as six.
-        replace (state_update IT s0X j s) with (proj1_sig six); try (subst; reflexivity).
-        apply (protocol_initial_state composite_vlsm_free).
+        remember (exist (@initial_state_prop _ _ S) (lift_to_composite_state i0 IS j s) Hinit) as six.
+        replace (lift_to_composite_state i0 IS j s) with (proj1_sig six); try (subst; reflexivity).
+        apply (protocol_initial_state free_composite_vlsm).
       - assert (Hinit : @initial_message_prop _ _ S (proj1_sig im)).
         { exists j. exists im. reflexivity. }
-        replace (state_update IT s0X j s) with s0X
+        replace (lift_to_composite_state i0 IS j s) with (proj1_sig (@Common.s0 _ _ S))
         ; try (symmetry; apply state_update_id; reflexivity).
-        unfold s in *; unfold om in *; clear s om.
+        unfold om in *; unfold s in *; clear s om.
         destruct im as [m _H]; simpl in *; clear _H.
         remember (exist (@initial_message_prop _ _ S) m Hinit) as im.
         replace m with (proj1_sig im); try (subst; reflexivity).
-        apply (protocol_initial_message composite_vlsm_free).
+        apply (protocol_initial_message free_composite_vlsm).
       - specialize (IHHp1 s _om eq_refl).
         specialize (IHHp2 _s om eq_refl).
-        replace (state_update IT s0X j sj, om0) with (@transition _ _ _ composite_vlsm_free (existT _ j l) (state_update IT s0X j s, om)).
-        + apply (protocol_generated composite_vlsm_free) with _om (state_update IT s0X j _s)
+        replace
+          (@pair (composite_state IT) (option message) (@lift_to_composite_state IT i0 IS j sj) om0)
+          with (@transition _ _ _ free_composite_vlsm (existT _ j l) (lift_to_composite_state i0 IS j s, om)).
+        + apply (protocol_generated free_composite_vlsm) with _om (lift_to_composite_state i0 IS j _s)
           ; try assumption.
           split; try exact I.
-          simpl. rewrite state_update_eq. assumption.
-        + simpl. rewrite state_update_eq. rewrite H0.
+          simpl. unfold lift_to_composite_state. rewrite state_update_eq. assumption.
+        + simpl. unfold lift_to_composite_state. rewrite state_update_eq. rewrite H0.
           f_equal.
           apply state_update_twice.
     Qed.
 
   End composite_vlsm.
 
-  Section composite_vlsm_decidable.
+End VLSM_composition.
 
-    Context {message : Type}
-            {index : Type}
-            {IndEqDec : EqDec index}
-            {IT : index -> VLSM_type message}
-            (i0 : index)
-            {IS : forall i : index, LSM_sig (IT i)}
-            {IM : forall n : index, VLSM (IS n)}
-            (IDM : forall n : index, VLSM_vdecidable (IM n)).
-
-    (* Composing decidable VLSMs *)
-
-    Definition _composite_valid_decidable
-               (l : composite_label IT)
-               (som : composite_state IT * option message)
-      : {_composite_valid IM l som} + {~_composite_valid IM l som}.
-      destruct som as [s om].
-      destruct l as [i li]; simpl.
-      apply (valid_decidable (IM i)).
-    Defined.
-
-    Definition _composite_valid_constrained_decidable
-               {constraint : composite_label IT -> composite_state IT * option message -> Prop}
-               (constraint_decidable : forall (l : composite_label IT) (som : composite_state IT * option (message)), {constraint l som} + {~constraint l som})
-               (l : composite_label IT)
-               (som : composite_state IT * option message)
-      : {composite_valid i0 IM constraint l som} + {~composite_valid i0 IM constraint l som}.
-      intros.
-      destruct (constraint_decidable l som) as [Hc | Hnc].
-      - destruct (_composite_valid_decidable l som) as [Hv | Hnv].
-        + left. split; try assumption.
-        + right. intros [Hv _]. contradiction.
-      - right. intros [_ Hc]. contradiction.
-    Defined.
-
-    Definition composite_vlsm_constrained_vdecidable
-               {constraint : composite_label IT -> composite_state IT * option message -> Prop}
-               (constraint_decidable : forall (l : composite_label IT) (som : composite_state IT * option (message)), {constraint l som} + {~constraint l som})
-      : VLSM_vdecidable (composite_vlsm_constrained i0 IM constraint)
-      :=
-        {|  valid_decidable := _composite_valid_constrained_decidable constraint_decidable
-        |}.
-
-    Definition composite_valid_constrained_decidable
-               {constraint : composite_label IT -> composite_state IT * option (message) -> Prop}
-               (constraint_decidable : forall (l : composite_label IT) (som : composite_state IT * option (message)), {constraint l som} + {~constraint l som})
-      := @valid_decidable _ _ _ _ (composite_vlsm_constrained_vdecidable constraint_decidable).
-
-    Definition free_constraint_decidable
-               (l : composite_label IT)
-               (som : composite_state IT * option (message))
-      : {free_constraint l som} + {~free_constraint l som}
-      := left I.
-
-    Definition composite_vlsm_free_vdecidable
-      : VLSM_vdecidable (composite_vlsm_free i0 IM)
-      :=
-        composite_vlsm_constrained_vdecidable free_constraint_decidable.
-
-  End composite_vlsm_decidable.
-End indexing.
-
-(* Section 2.4.4 Projections into VLSM compositions *)
 Section projections.
+(**
+* Composite VLSM projections
+
+Let us fix an indexed set of VLSMs <<IM>> and their composition <<X>> using <<constraint>>.
+
+*)
 
   Context {message : Type}
           {index : Type}
           {IndEqDec : EqDec index}
           (i0 : index)
           {IT : index -> VLSM_type message}
-          {IS : forall i : index, LSM_sig (IT i)}
+          {IS : forall i : index, VLSM_sign (IT i)}
           (IM : forall n : index, VLSM (IS n))
           (T := composite_type IT)
           (S := composite_sig i0 IS)
           (constraint : @label _ T -> @state _ T * option message -> Prop)
-          (X := composite_vlsm_constrained i0 IM constraint)
+          (X := composite_vlsm i0 IM constraint)
           .
 
-  Definition composite_vlsm_constrained_projection_sig (i : index) : LSM_sig (IT i)
+(**
+The [VLSM_type] of a projection of <<X>> to component <<i>> is <<IT i>>, the
+type of the <<i>>th component of <<X>>.
+We defined the signature of the projection to be the same as that of the component,
+with the exception that the [initial_message]s for the projection are defined
+to be all [protocol_message]s of <<X>>:
+
+*)
+  Definition composite_vlsm_constrained_projection_sig (i : index) : VLSM_sign (IT i)
     :=
       {|      initial_state_prop := @initial_state_prop _ _ (IS i)
           ;   initial_message_prop := fun pmi => exists xm : (@protocol_message _ _ _ X), proj1_sig xm = pmi
@@ -412,6 +482,10 @@ Section projections.
           ;   m0 := @m0 _ _ (IS i)
           ;   l0 := @l0 _ _ (IS i)
       |}.
+
+(**
+[projection_valid]ity is defined as the projection of [protocol_valid]ity of <<X>>:
+*)
 
   Definition projection_valid
     (i : index)
@@ -423,7 +497,12 @@ Section projections.
       s i = si /\ protocol_valid X (existT _ i li) (s, omi)
     .
 
-  Lemma composite_protocol_valid_implies_valid
+(**
+Since [projection_valid]ity is derived from [protocol_valid]ity, which in turn
+depends on [valid]ity in the component, it is easy to see that
+[projection_valid]ity implies [valid]ity in the component.
+*)
+  Lemma projection_valid_implies_valid
     (i : index)
     (li : @label _ (IT i))
     (siomi : @state _ (IT i) * option message)
@@ -435,9 +514,14 @@ Section projections.
     destruct Hcomposite as [s [Hsi [_ [_ Hvalid]]]].
     subst; simpl in *.
     destruct Hvalid as [Hvalid Hconstraint].
-    unfold _composite_valid in Hvalid. assumption.
+    assumption.
   Qed.
 
+(**
+We define the projection of <<X>> to index <<i>> as the [VLSM] whose signature
+is the [composite_vlsm_constrained_projection_sig]nature corresponding to <<i>>,
+having the same transition function as <<IM i>>, the <<i>>th component of 
+*)
   Definition composite_vlsm_constrained_projection
              (i : index)
     : VLSM (composite_vlsm_constrained_projection_sig i) :=
@@ -446,47 +530,73 @@ Section projections.
     |}.
 
   Section fixed_projection.
+
+(**
+
+** Projection traces are Byzantine
+
+Let us fix an index <<j>> and let <<Xj>> be the projection of <<X>> on
+component <<j>>.
+
+In this section we establish some basic properties for projections, building up
+to Lemma [proj_pre_loaded_incl], which guarantees that all
+[protocol_trace]s of <<Xj>> are also [protocol_trace]s for the
+[pre_loaded_vlsm] associated to the component <<IM j>>.
+In particular this ensures that the byzantine traces of <<IM j>> include all
+[protocol_trace]s of <<Xj>> (see Lemma [pre_loaded_alt_eq]).
+
+*)
   
     Context
       (j : index)
-      (Proj := composite_vlsm_constrained_projection j)
+      (Xj := composite_vlsm_constrained_projection j)
       .
-  
+
+(**
+As a basic property of the definition of initial states it follows that
+the <<j>>th component of an [initial_state] of <<X>> is initial for <<Xj>>
+*)
+
     Lemma initial_state_projection
       (s : @state _ T)
       (Hinit : @initial_state_prop _ _ S s)
-      : @initial_state_prop _ _ (sign Proj) (s j)
+      : @initial_state_prop _ _ (sign Xj) (s j)
       .
     Proof.
       specialize (Hinit j).
       assumption.
     Qed.
-  
-    Lemma transition_projection : @transition _ _ (composite_vlsm_constrained_projection_sig j) Proj = @transition _ _ _ (IM j).
-    Proof. reflexivity.  Qed.
-  
+
+(**
+Since all [protocol_message]s of <<X>> become [initial_message]s in <<Xj>>, the
+following result is not surprising.
+*)
     Lemma protocol_message_projection
       (iom : option message)
-      (HpmX : exists sx : state, protocol_prop X (sx, iom))
-      : exists sj : state, protocol_prop Proj (sj, iom)
+      (HpmX : option_protocol_message_prop X iom)
+      : option_protocol_message_prop Xj iom
       .
     Proof.
       exists (proj1_sig s0).
       destruct iom as [im|].
-      - specialize (protocol_initial_message Proj ); intro Hinit.
+      - specialize (protocol_initial_message Xj ); intro Hinit.
         assert (Hpim : protocol_message_prop X im)
           by assumption.
-        assert (Hini : @initial_message_prop _ _ (sign Proj) im)
+        assert (Hini : @initial_message_prop _ _ (sign Xj) im)
           by (exists (exist _ im Hpim); reflexivity).
         specialize (Hinit (exist _ im Hini)); simpl in Hinit.
         assumption.
-      - apply (protocol_initial_state Proj).
+      - apply (protocol_initial_state Xj).
     Qed.
   
+(**
+Interestingly enough, <<Xj>> cannot produce any additional messages than
+the initial ones available from <<X>>.
+*)
     Lemma protocol_message_projection_rev
       (iom : option message)
-      (Hpmj: exists sj : state, protocol_prop Proj (sj, iom))
-      : exists sx : state, protocol_prop X (sx, iom)
+      (Hpmj: option_protocol_message_prop Xj iom)
+      : option_protocol_message_prop X iom
       .
     Proof.
       destruct Hpmj as [sj Hpmj].
@@ -515,11 +625,16 @@ Section projections.
         assumption.
     Qed.
 
+(**
+As a stepping stone towards proving trace inclusion between <<Xj>> and
+the [pre_loaded_vlsm] associated to <<IM j>>, we prove that the
+[protocol_prop]erty is transferred.
+*)
     Lemma proj_pre_loaded_protocol_prop
       (PreLoaded := pre_loaded_vlsm (IM j))
       (s : state)
       (om : option message)
-      (Hps : protocol_prop Proj (s, om))
+      (Hps : protocol_prop Xj (s, om))
       : protocol_prop PreLoaded (s, om).
     Proof.
       induction Hps.
@@ -529,20 +644,23 @@ Section projections.
           by exact I.
         apply (protocol_initial_message PreLoaded (exist _ m Him)).
       - apply (protocol_generated PreLoaded) with _om _s; try assumption.
-        apply composite_protocol_valid_implies_valid. assumption.
+        apply projection_valid_implies_valid. assumption.
     Qed.
-    
+
+(**
+We can now finally prove the main result for this section:
+*)
     Lemma proj_pre_loaded_incl
       (PreLoaded := pre_loaded_vlsm (IM j))
-      : VLSM_incl Proj PreLoaded
+      : VLSM_incl Xj PreLoaded
       .
     Proof.
-      apply (basic_VLSM_incl Proj PreLoaded)
+      apply (basic_VLSM_incl Xj PreLoaded)
       ; intros; try (assumption || reflexivity).
       - destruct H as [_ [[_s Hpm] _]]. exists _s.
         apply proj_pre_loaded_protocol_prop.
         assumption.
-      - apply composite_protocol_valid_implies_valid.
+      - apply projection_valid_implies_valid.
         destruct H as [_ [_ Hv]].
         assumption.
     Qed.
@@ -552,20 +670,29 @@ Section projections.
 End projections.
 
 Section free_projections.
+(**
+
+** Projections of free compositions
+
+These projections are simple instances of the projections defined above in which
+the composition constraint is taken to be [True].
+
+All results from regular projections carry to these "free" projections.
+*)
 
   Context {message : Type}
           {index : Type}
           {IndEqDec : EqDec index}
           (i0 : index)
           {IT : index -> VLSM_type message}
-          {IS : forall i : index, LSM_sig (IT i)}
+          {IS : forall i : index, VLSM_sign (IT i)}
           (IM : forall n : index, VLSM (IS n))
-          (X := composite_vlsm_free i0 IM)
+          (X := free_composite_vlsm i0 IM)
           .
 
   Definition composite_vlsm_free_projection_sig
              (i : index)
-    : LSM_sig (IT i)
+    : VLSM_sign (IT i)
     :=
       composite_vlsm_constrained_projection_sig i0 IM free_constraint i.
 
@@ -577,12 +704,23 @@ Section free_projections.
 
 End free_projections.
 
-Section binary_composition.
+Section binary_free_composition.
+
+(**
+
+* Free composition of two VLSMs
+
+This serves an example of how composition can be built, but is also being
+used in definiting the [byzantine_trace_prop]erties.
+
+This instantiates the regular composition using the [bool] type as an <<index>>.
+
+*)
   Context
     {message : Type}
     {T1 T2 : VLSM_type message}
-    {S1 : LSM_sig T1}
-    {S2 : LSM_sig T2}
+    {S1 : VLSM_sign T1}
+    {S2 : VLSM_sign T2}
     (M1 : VLSM S1)
     (M2 : VLSM S2)
     .
@@ -592,24 +730,28 @@ Section binary_composition.
   Definition first : binary_index := true.
   Definition second : binary_index := false.
 
-  Program Instance binary_index_dec :  EqDec binary_index := bool_dec.
+  Global Instance binary_index_dec :  EqDec binary_index := bool_dec.
 
   Definition binary_IT
     (i : binary_index)
     :=
     match i with
-    | true => T1
-    | false => T2
+    | true => (type M1)
+    | false => (type M2)
     end.
 
-  Definition binary_IS (i : binary_index) : LSM_sig (binary_IT i)
+  Definition binary_IS
+    (i : binary_index)
+    : VLSM_sign (binary_IT i)
     :=
     match i with
     | true => S1
     | false => S2
     end.
 
-  Definition binary_IM (i : binary_index) : VLSM (binary_IS i)
+  Definition binary_IM
+    (i : binary_index)
+    : VLSM (binary_IS i)
     :=
     match i with
     | true => M1
@@ -618,7 +760,7 @@ Section binary_composition.
 
   Definition binary_free_composition
     : VLSM (composite_sig first binary_IS)
-    := composite_vlsm_free first binary_IM.
+    := free_composite_vlsm first binary_IM.
 
   Definition binary_free_composition_fst
     := composite_vlsm_free_projection first binary_IM  first.
@@ -626,4 +768,4 @@ Section binary_composition.
   Definition binary_free_composition_snd
     := composite_vlsm_free_projection first binary_IM  second.
 
-End binary_composition.
+End binary_free_composition.
